code/poly1305/Hacl.Impl.Poly1305.Lemmas.fst
@@ -7,64 +7,30 @@ open Lib.IntVector
 open Lib.Sequence
 open Lib.ByteSequence
 
-friend Lib.ByteSequence
-
-let lemma_cast_vec128_to_vec64 b = cast_vec_u128_to_u64_lemma b
-
-let lemma_cast_vec64_to_vec128 b = cast_vec_u64_to_u128_lemma #2 b
-
-let lemma_vec_interleave_low_cast_64_4 b1 b2 =
-  let r1 = cast U128 2 b1 in
-  lemma_cast_vec64_to_vec128 b1;
-  let r2 = cast U128 2 b2 in
-  lemma_cast_vec64_to_vec128 b2;
-  let r3 = vec_interleave_low r1 r2 in
-  vec_interleave_low_lemma2 r1 r2;
-  let r4 = cast U64 4 r3 in
-  lemma_cast_vec128_to_vec64 r3;
-  uintv_extensionality (vec_v r4).[0] (vec_v b1).[0];
-  uintv_extensionality (vec_v r4).[1] (vec_v b1).[1];
-  uintv_extensionality (vec_v r4).[2] (vec_v b2).[0];
-  uintv_extensionality (vec_v r4).[3] (vec_v b2).[1];
-  eq_intro (vec_v r4) (create4 (vec_v b1).[0] (vec_v b1).[1] (vec_v b2).[0] (vec_v b2).[1])
-
-let lemma_vec_interleave_high_cast_64_4 b1 b2 =
-  let r1 = cast U128 2 b1 in
-  lemma_cast_vec64_to_vec128 b1;
-  let r2 = cast U128 2 b2 in
-  lemma_cast_vec64_to_vec128 b2;
-  let r3 = vec_interleave_high r1 r2 in
-  vec_interleave_high_lemma2 r1 r2;
-  let r4 = cast U64 4 r3 in
-  lemma_cast_vec128_to_vec64 r3;
-  uintv_extensionality (vec_v r4).[0] (vec_v b1).[2];
-  uintv_extensionality (vec_v r4).[1] (vec_v b1).[3];
-  uintv_extensionality (vec_v r4).[2] (vec_v b2).[2];
-  uintv_extensionality (vec_v r4).[3] (vec_v b2).[3];
-  eq_intro (vec_v r4) (create4 (vec_v b1).[2] (vec_v b1).[3] (vec_v b2).[2] (vec_v b2).[3])
-
 #set-options "--z3rlimit 50 --max_fuel 1"
 
 let uint_from_bytes_le_lemma b =
   let r1 = nat_from_bytes_le b in
-  uints_from_bytes_le_nat_lemma #U64 #_ #2 b;
-  assert (r1 == nat_from_intseq_le_ (uints_from_bytes_le #U64 #_ #2 b));
-  let r2 = uints_from_bytes_le #U64 #_ #2 b in
-  assert (r2.[0] == uint_from_bytes_le (sub b 0 8));
-  assert (r2.[1] == uint_from_bytes_le (sub b 8 8));
-  assert (nat_from_intseq_le_ r2 == v r2.[0] + pow2 64 * nat_from_intseq_le_ (Seq.slice r2 1 2));
-  assert (nat_from_intseq_le_ (Seq.slice r2 1 2) == v r2.[1])
-  
+  let r2 = uints_from_bytes_le #U64 #SEC #2 b in
+  uints_from_bytes_le_nat_lemma #U64 #SEC #2 b;
+  assert (r1 == nat_from_intseq_le r2);
+  nat_from_intseq_le_slice_lemma #U64 #SEC #2 r2 1;
+  assert (r1 == nat_from_intseq_le (Seq.slice r2 0 1) + pow2 64 * nat_from_intseq_le #U64 #SEC (Seq.slice r2 1 2));
+  nat_from_intseq_le_lemma0 (Seq.slice r2 0 1);
+  nat_from_intseq_le_lemma0 (Seq.slice r2 1 2);
+  assert (r1 == uint_v r2.[0] + pow2 64 * uint_v r2.[1]);
+  Classical.forall_intro (index_uints_from_bytes_le #U64 #SEC #2 b)
+
 let uints_from_bytes_le_lemma64_1 b =
+  index_uints_from_bytes_le #U64 #SEC #1 (sub b 0 8) 0;
+  index_uints_from_bytes_le #U64 #SEC #1 (sub b 8 8) 0;
   uint_from_bytes_le_lemma b
 
 let uints_from_bytes_le_lemma64_2 b =
+  Classical.forall_intro (index_uints_from_bytes_le #U64 #SEC #2 (sub b 0 16));
+  Classical.forall_intro (index_uints_from_bytes_le #U64 #SEC #2 (sub b 16 16));
   uint_from_bytes_le_lemma (sub b 0 16);
   uint_from_bytes_le_lemma (sub b 16 16)
-
-let uints_from_bytes_le_lemma128_2 b = ()
-
-let uint_to_bytes_le_lemma128 r = ()
 
 module BF = Vale.Arch.BufferFriend
 
@@ -100,31 +66,28 @@ let uints_to_bytes_le_lemma64_2 r =
   // lemmas to prove this simply.
   admit ()
 
-let uints_to_bytes_le_lemma128_2 r =
-  // ibid.
-  admit ()
-
-#push-options "--initial_fuel 1 --max_fuel 1 --max_ifuel 0"
 val lemma_nat_from_bytes_le_zeroes: len:size_nat -> b:lseq uint8 len -> Lemma
   (requires (forall (i:nat). i < len ==> b.[i] == u8 0))
-  (ensures  nat_from_intseq_le_ b == 0)
+  (ensures  nat_from_intseq_le b == 0)
 let rec lemma_nat_from_bytes_le_zeroes len b =
   if len = 0 then ()
-  else lemma_nat_from_bytes_le_zeroes (len-1) (Seq.slice b 1 len)
-#pop-options
+  else begin
+    nat_from_intseq_le_slice_lemma #U8 #SEC #len b 1;
+    nat_from_intseq_le_lemma0 (Seq.slice b 0 1);
+    lemma_nat_from_bytes_le_zeroes (len-1) (Seq.slice b 1 len) end
 
 val nat_from_bytes_le_eq_lemma_: len:size_nat{len < 16} -> b:lseq uint8 len -> Lemma
  (let tmp = create 16 (u8 0) in
-  BSeq.nat_from_intseq_le_ b == BSeq.nat_from_intseq_le_ (update_sub tmp 0 len b))
+  BSeq.nat_from_intseq_le b == BSeq.nat_from_intseq_le (update_sub tmp 0 len b))
 let nat_from_bytes_le_eq_lemma_ len b =
   let tmp = create 16 (u8 0) in
   let r = update_sub tmp 0 len b in
   assert (Seq.slice r 0 len == b);
   assert (forall (i:nat). len <= i /\ i < 16 ==> r.[i] == u8 0);
   assert (forall (i:nat). i < 16 - len ==> Seq.index (Seq.slice r len 16) i == u8 0);
-  nat_from_bytes_le_slice_lemma #_ #16 r len;
-  assert (nat_from_intseq_le_ r == nat_from_intseq_le_ (Seq.slice r 0 len) + pow2 (len * 8) * nat_from_intseq_le_ (Seq.slice r len 16));
-  assert (nat_from_intseq_le_ r == nat_from_intseq_le_ b + pow2 (len * 8) * nat_from_intseq_le_ (Seq.slice r len 16));
+  nat_from_intseq_le_slice_lemma #U8 #SEC #16 r len;
+  assert (nat_from_intseq_le r == nat_from_intseq_le (Seq.slice r 0 len) + pow2 (len * 8) * nat_from_intseq_le (Seq.slice r len 16));
+  assert (nat_from_intseq_le r == nat_from_intseq_le b + pow2 (len * 8) * nat_from_intseq_le (Seq.slice r len 16));
   lemma_nat_from_bytes_le_zeroes (16 - len) (Seq.slice r len 16)
 
 let nat_from_bytes_le_eq_lemma len b = nat_from_bytes_le_eq_lemma_ len b
