code/poly1305/Hacl.Poly1305.Field32xN.Lemmas.fst
@@ -8,7 +8,7 @@ open FStar.Mul
 open Hacl.Spec.Poly1305.Vec
 include Hacl.Spec.Poly1305.Field32xN
 
-#reset-options "--z3rlimit 20 --using_facts_from '* -FStar.Seq' --max_fuel 0 --max_ifuel 0"
+#reset-options "--z3rlimit 50 --using_facts_from '* -FStar.Seq' --max_fuel 0 --max_ifuel 0"
 
 val lemma_prime: unit ->
   Lemma (pow2 130 % prime = 5)
@@ -623,11 +623,11 @@ let precomp_r5_as_tup64 #w r i =
   FStar.Math.Lemmas.modulo_lemma (5 * v tr2) (pow2 64);
   FStar.Math.Lemmas.modulo_lemma (5 * v tr3) (pow2 64);
   FStar.Math.Lemmas.modulo_lemma (5 * v tr4) (pow2 64);
-  uintv_extensionality tr50 (tr0 *! u64 5);
-  uintv_extensionality tr51 (tr1 *! u64 5);
-  uintv_extensionality tr52 (tr2 *! u64 5);
-  uintv_extensionality tr53 (tr3 *! u64 5);
-  uintv_extensionality tr54 (tr4 *! u64 5)
+  assert (v tr50 == v (tr0 *! u64 5));
+  assert (v tr51 == v (tr1 *! u64 5));
+  assert (v tr52 == v (tr2 *! u64 5));
+  assert (v tr53 == v (tr3 *! u64 5));
+  assert (v tr54 == v (tr4 *! u64 5))
 
 val mul_felem5_eval_as_tup64:
     #w:lanes
@@ -700,7 +700,7 @@ let carry26_wide_lemma_i #w #m l cin i =
   let l0 = l' &. mask26 in
   let l1 = l' >>. 26ul in
   mod_mask_lemma l' 26ul;
-  uintv_extensionality (mod_mask #U64 26ul) mask26;
+  assert (v (mod_mask #U64 #SEC 26ul) == v mask26);
   FStar.Math.Lemmas.pow2_modulo_modulo_lemma_1 (v l') 26 32;
   FStar.Math.Lemmas.euclidean_division_definition (v l') (pow2 26)
 
@@ -805,7 +805,7 @@ let carry26_lemma_i #w l cin i =
   let l0 = l' &. mask26 in
   let l1 = l' >>. 26ul in
   mod_mask_lemma l' 26ul;
-  uintv_extensionality (mod_mask #U64 26ul) mask26;
+  assert (v (mod_mask #U64 #SEC 26ul) == v mask26);
   FStar.Math.Lemmas.pow2_modulo_modulo_lemma_1 (v l') 26 32;
   FStar.Math.Lemmas.pow2_minus 32 26
 
@@ -1117,7 +1117,7 @@ let carry_reduce_lemma_i #w l cin i =
   let li0 = li' &. mask26 in
   let li1 = li' >>. 26ul in
   mod_mask_lemma li' 26ul;
-  uintv_extensionality (mod_mask #U64 26ul) mask26;
+  assert (v (mod_mask #U64 #SEC 26ul) == v mask26);
   FStar.Math.Lemmas.pow2_modulo_modulo_lemma_1 (v li') 26 32;
   FStar.Math.Lemmas.pow2_minus 32 26
 
@@ -1372,23 +1372,36 @@ val load_tup64_lemma0_lo: lo:uint64 ->
     (v lo % pow2 26 + ((v lo / pow2 26) % pow2 26) * pow26 +
     v lo / pow2 52 * pow26 * pow26 == v lo)
 let load_tup64_lemma0_lo lo =
-  assert_norm (pow26 = pow2 26);
-  assert_norm (pow26 * pow26 = pow2 52);
-  FStar.Math.Lemmas.pow2_modulo_division_lemma_1 (v lo) 26 52;
-  assert (v lo % pow2 26 == (v lo % pow2 52) % pow2 26);
-  FStar.Math.Lemmas.euclidean_division_definition (v lo % pow2 52) (pow2 26);
-  FStar.Math.Lemmas.euclidean_division_definition (v lo) (pow2 52)
+  calc (==) {
+    v lo % pow2 26 + ((v lo / pow2 26) % pow2 26) * pow26 + v lo / pow2 52 * pow26 * pow26;
+  (==) { assert_norm (pow26 * pow26 = pow2 52) }
+    v lo % pow2 26 + ((v lo / pow2 26) % pow2 26) * pow2 26 + v lo / pow2 52 * pow2 52;
+  (==) { FStar.Math.Lemmas.pow2_modulo_modulo_lemma_1 (v lo) 26 52 }
+    (v lo % pow2 52) % pow2 26 + ((v lo / pow2 26) % pow2 26) * pow2 26 + v lo / pow2 52 * pow2 52;
+  (==) { FStar.Math.Lemmas.pow2_modulo_division_lemma_1 (v lo) 26 52 }
+    (v lo % pow2 52) % pow2 26 + ((v lo % pow2 52) / pow2 26) * pow2 26 + v lo / pow2 52 * pow2 52;
+  (==) { FStar.Math.Lemmas.euclidean_division_definition (v lo % pow2 52) (pow2 26) }
+    (v lo % pow2 52) + v lo / pow2 52 * pow2 52;
+  (==) { FStar.Math.Lemmas.euclidean_division_definition (v lo) (pow2 52) }
+    v lo;
+  }
 
 val load_tup64_lemma0_hi: hi:uint64 ->
   Lemma
     (v hi % pow2 14 + ((v hi / pow2 14) % pow2 26) * pow2 14 +
     (v hi / pow2 40) * pow2 40 == v hi)
 let load_tup64_lemma0_hi hi =
-  FStar.Math.Lemmas.pow2_modulo_division_lemma_1 (v hi) 14 40;
-  FStar.Math.Lemmas.pow2_modulo_modulo_lemma_1 (v hi) 14 40;
-  assert (v hi % pow2 14 == (v hi % pow2 40) % pow2 14);
-  FStar.Math.Lemmas.euclidean_division_definition (v hi % pow2 40) (pow2 14);
-  FStar.Math.Lemmas.euclidean_division_definition (v hi) (pow2 40)
+  calc (==) {
+    v hi % pow2 14 + ((v hi / pow2 14) % pow2 26) * pow2 14 + (v hi / pow2 40) * pow2 40;
+  (==) { FStar.Math.Lemmas.pow2_modulo_division_lemma_1 (v hi) 14 40 }
+    v hi % pow2 14 + ((v hi % pow2 40) / pow2 14) * pow2 14 + (v hi / pow2 40) * pow2 40;
+  (==) { FStar.Math.Lemmas.pow2_modulo_modulo_lemma_1 (v hi) 14 40 }
+    (v hi % pow2 40) % pow2 14 + ((v hi % pow2 40) / pow2 14) * pow2 14 + (v hi / pow2 40) * pow2 40;
+  (==) { FStar.Math.Lemmas.euclidean_division_definition (v hi % pow2 40) (pow2 14) }
+    v hi % pow2 40 + (v hi / pow2 40) * pow2 40;
+  (==) { FStar.Math.Lemmas.euclidean_division_definition (v hi) (pow2 40) }
+    v hi;
+  }
 
 val load_tup64_lemma0:
     f:tup64_5
@@ -1461,7 +1474,7 @@ let load_tup64_lemma lo hi =
 
   let f0 = lo &. mask26 in
   mod_mask_lemma lo 26ul;
-  uintv_extensionality (mod_mask #U64 26ul) mask26;
+  assert (v (mod_mask #U64 #SEC 26ul) == v mask26);
   assert (v f0 == v lo % pow2 26);
 
   let f1 = (lo >>. 26ul) &. mask26 in
@@ -1470,7 +1483,7 @@ let load_tup64_lemma lo hi =
   let f2 = (lo >>. 52ul) |. ((hi &. u64 0x3fff) <<. 12ul) in
   FStar.Math.Lemmas.lemma_div_lt (v lo) 64 52;
   mod_mask_lemma hi 14ul;
-  uintv_extensionality (mod_mask #U64 14ul) (u64 0x3fff);
+  assert (v (mod_mask #U64 #SEC 14ul) == v (u64 0x3fff));
   FStar.Math.Lemmas.pow2_multiplication_modulo_lemma_1 (v hi % pow2 14) 12 12;
   assert ((v (lo >>. 52ul)) < pow2 12);
   [@inline_let] let tmp = (hi &. u64 0x3fff) in
@@ -1541,6 +1554,9 @@ let lemma_store_felem_lo f lo =
   let (f0, f1, f2, f3, f4) = f in
   assert_norm (max26 = pow2 26 - 1);
   let lo = f0 |. (f1 <<. 26ul) |. (f2 <<. 52ul) in
+  assert (v (f1 <<. 26ul) == v f1 * pow2 26 % pow2 64);
+  assert_norm (pow2 26 * pow2 26 = pow2 52);
+  FStar.Math.Lemmas.modulo_lemma (v f1 * pow2 26) (pow2 64);
   FStar.Math.Lemmas.pow2_multiplication_modulo_lemma_1 (v f1) 26 26;
   logor_disjoint f0 (f1 <<. 26ul) 26;
   assert (v (f0 |. (f1 <<. 26ul)) == v f0 + v f1 * pow2 26);
@@ -1562,6 +1578,9 @@ let lemma_store_felem_hi f hi =
   let hi = (f2 >>. 12ul) |. (f3 <<. 14ul) |. (f4 <<. 40ul) in
   FStar.Math.Lemmas.lemma_div_lt (v f2) 26 12;
   assert (v f2 / pow2 12 < pow2 14);
+
+  assert (v (f3 <<. 14ul) == v f3 * pow2 14 % pow2 64);
+  FStar.Math.Lemmas.lemma_mult_le_right (pow2 14) (v f3) (pow2 26);
   assert_norm (pow2 26 * pow2 14 = pow2 40);
   assert_norm (pow2 40 < pow2 64);
   FStar.Math.Lemmas.modulo_lemma (v f3 * pow2 14) (pow2 64);
@@ -1673,21 +1692,18 @@ let store_tup64_lemma f =
   lemma_tup64_as_nat (f0, f1, f2, f3, u64 (v f4 % pow2 24));
   lo, hi
 
-val store_felem5_lemma_i:
+val store_felem5_lemma:
     #w:lanes
   -> f:felem5 w
-  -> i:nat{i < w}
   -> Lemma
     (requires felem_fits5 f (1, 1, 1, 1, 1))
     (ensures
       (let (lo, hi) = store_felem5 f in
-      (uint64xN_v hi).[i] * pow2 64 + (uint64xN_v lo).[i] == (fas_nat5 f).[i] % pow2 128))
+      v hi * pow2 64 + v lo == (fas_nat5 f).[0] % pow2 128))
 #push-options "--max_ifuel 1"
-let store_felem5_lemma_i #w f i =
+let store_felem5_lemma #w f =
   let (lo, hi) = store_felem5 f in
-  let loi = (vec_v lo).[i] in
-  let hii = (vec_v hi).[i] in
-  assert (store_tup64_lemma (as_tup64_i f i) == (loi, hii))
+  assert (store_tup64_lemma (as_tup64_i f 0) == (lo, hi))
 #pop-options
 
 #push-options "--z3rlimit 200"
@@ -1905,17 +1921,14 @@ let add_mod_small a b n =
   FStar.Math.Lemmas.lemma_mod_plus_distr_l a (b % n) n;
   FStar.Math.Lemmas.lemma_mod_plus_distr_r a b n
 
-val mod_add128_sc:
+val mod_add128_lemma:
     a:(uint64 & uint64)
-  -> b:(uint64 & uint64)
-  -> Pure (uint64 & uint64)
-    (requires True)
-    (ensures fun (r0, r1) ->
-     let (a0, a1) = a in
-     let (b0, b1) = b in
-     v r1 * pow2 64 + v r0 ==
-     ((v a1 + v b1) * pow2 64 + v a0 + v b0) % pow2 128)
-let mod_add128_sc a b =
+  -> b:(uint64 & uint64) ->
+  Lemma (
+    let (r0, r1) = mod_add128 a b in
+    let (a0, a1) = a in let (b0, b1) = b in
+    v r1 * pow2 64 + v r0 == ((v a1 + v b1) * pow2 64 + v a0 + v b0) % pow2 128)
+let mod_add128_lemma a b =
   let (a0, a1) = a in
   let (b0, b1) = b in
   let r0 = a0 +. b0 in
@@ -1952,27 +1965,4 @@ let mod_add128_sc a b =
   add_mod_small ((v a1 + v b1) * pow2 64 + (v a0 + v b0) / pow2 64 * pow2 64) ((v a0 + v b0) % pow2 64) (pow2 128);
   assert (v r2 * pow2 64 + v r0 == ((v a1 + v b1) * pow2 64 + (v a0 + v b0) / pow2 64 * pow2 64 + (v a0 + v b0) % pow2 64) % pow2 128);
   FStar.Math.Lemmas.euclidean_division_definition (v a0 + v b0) (pow2 64);
-  assert (v r2 * pow2 64 + v r0 == ((v a1 + v b1) * pow2 64 + v a0 + v b0) % pow2 128);
-  (r0, r2)
-
-val mod_add128_lemma_i:
-    #w:lanes
-  -> a:(uint64xN w & uint64xN w)
-  -> b:(uint64xN w & uint64xN w)
-  -> i:nat{i < w}
-  -> Lemma
-    (let (r0, r1) = mod_add128_ws a b in
-     let (a0, a1) = a in
-     let (b0, b1) = b in
-    (uint64xN_v r1).[i] * pow2 64 + (uint64xN_v r0).[i] ==
-      (((uint64xN_v a1).[i] + (uint64xN_v b1).[i]) * pow2 64 +
-      (uint64xN_v a0).[i] + (uint64xN_v b0).[i]) % pow2 128)
-let mod_add128_lemma_i #w a b i =
-  let (a0, a1) = a in
-  let (b0, b1) = b in
-  let (r0, r1) = mod_add128_ws a b in
-  let (a0i, a1i) = ((vec_v a0).[i], (vec_v a1).[i]) in
-  let (b0i, b1i) = ((vec_v b0).[i], (vec_v b1).[i]) in
-
-  let r0s, r1s = mod_add128_sc (a0i, a1i) (b0i, b1i) in
-  assert ((vec_v r0).[i] == r0s /\ (vec_v r1).[i] == r1s)
+  assert (v r2 * pow2 64 + v r0 == ((v a1 + v b1) * pow2 64 + v a0 + v b0) % pow2 128)
