code/tests/Hacl.Test.SHA3.fst
@@ -10,7 +10,7 @@ open Lib.Buffer
 open Lib.PrintBuffer
 open Hacl.SHA3
 
-#reset-options "--z3rlimit 50 --max_fuel 0 --max_ifuel 0 --using_facts_from '* -FStar.Seq'"
+#reset-options "--z3rlimit 100 --max_fuel 0 --max_ifuel 0 --using_facts_from '* -FStar.Seq'"
 
 val test_sha3:
     msg_len:size_t
